ref_impl/src/verifier/fstar_files/NSMain__main_main.fst
@@ -5,9 +5,9 @@ open BosqueTerms
 
 (* Type names *)
 let bTypedStringType_BAnyType = (BTypedStringType BAnyType)
+let bTypedStringType_BNoneType = (BTypedStringType BNoneType)
 let bTupleType_2BIntType_BIntTypefalse = BTupleType false 2 (SCons BIntType 1 (SCons BIntType 0 SNil))
 let bTupleType_16BIntType_BIntType_BIntType_BIntType_BIntType_BIntType_BIntType_BIntType_BIntType_BIntType_BIntType_BIntType_bTupleType_2BIntType_BIntTypefalse_bTypedStringType_BAnyType_BBoolType_BBoolTypefalse = BTupleType false 16 (SCons BIntType 15 (SCons BIntType 14 (SCons BIntType 13 (SCons BIntType 12 (SCons BIntType 11 (SCons BIntType 10 (SCons BIntType 9 (SCons BIntType 8 (SCons BIntType 7 (SCons BIntType 6 (SCons BIntType 5 (SCons BIntType 4 (SCons bTupleType_2BIntType_BIntTypefalse 3 (SCons bTypedStringType_BAnyType 2 (SCons BBoolType 1 (SCons BBoolType 0 SNil))))))))))))))))
-let bTypedStringType_BNoneType = (BTypedStringType BNoneType)
 let bUnionType_BBoolType_BIntType_BNoneType_bTypedStringType_BNoneType = (BUnionType BBoolType (BUnionType BIntType (BUnionType BNoneType bTypedStringType_BNoneType)))
 let bUnionType_BIntType_BNoneType = (BUnionType BIntType BNoneType)
 let bTupleType_3BIntType_BBoolType_BIntTypefalse = BTupleType false 3 (SCons BIntType 2 (SCons BBoolType 1 (SCons BIntType 0 SNil)))
@@ -35,15 +35,15 @@ let nSMain__identityUnion x =
 
 val nSMain__max : (x:bosqueTerm{subtypeOf bUnionType_BIntType_BNoneType (getType x)}) -> (x:bosqueTerm{subtypeOf BIntType (getType x)}) -> Tot (x:bosqueTerm{subtypeOf BIntType (getType x)})
 let nSMain__max x y = 
-  let __tmp_0 = true in 
-    if (op_Equality __tmp_0 true) then 
+  let __tmp_0 = (BBool true) in 
+    if (op_Equality __tmp_0 (BBool true)) then 
       let __ir_ret___2 = y in 
         let __ir_ret___3 = __ir_ret___2 in 
           let _return_ = __ir_ret___3 in 
             _return_
     else 
-      let __tmp_4 = (op_greaterOrEq x y) in 
-        if (op_Equality (extractBool __tmp_4) true) then 
+      let __tmp_4 = (extractBool (op_greaterOrEq x y)) in 
+        if (op_Equality __tmp_4 (BBool true)) then 
           let __ir_ret___1 = x in 
             let __ir_ret___3 = __ir_ret___1 in 
               let _return_ = __ir_ret___3 in 
@@ -68,8 +68,8 @@ let nSMain__identityOpenTuple x =
 
 val nSMain__maxx : (x:bosqueTerm{subtypeOf bUnionType_BBoolType_BNoneType (getType x)}) -> (x:bosqueTerm{subtypeOf BIntType (getType x)}) -> Tot (x:bosqueTerm{subtypeOf bUnionType_BBoolType_BIntType_BNoneType (getType x)})
 let nSMain__maxx x y = 
-  let __tmp_0 = (op_greater y 0) in 
-    if (op_Equality __tmp_0 true) then 
+  let __tmp_0 = (extractBool (op_greater y (BInt 0))) in 
+    if (op_Equality __tmp_0 (BBool true)) then 
       let __ir_ret___1 = x in 
         let __ir_ret___2 = __ir_ret___1 in 
           let _return_ = __ir_ret___2 in 
@@ -82,34 +82,43 @@ let nSMain__maxx x y =
 
 val nSMain__main : (x:bosqueTerm{subtypeOf BIntType (getType x)})
 let nSMain__main  = 
-  let string_test = "string_test" in 
-    let _LoadConstTypeString = 0 in 
-      let player1 = __tmp_1 in 
-        let n = none in 
-          let __tmp_3 = (Mktuple__2 10 30) in 
-            let xTuple2 = __tmp_3 in 
-              let __tmp_19 = (Mktuple__2 1 1) in 
-                let __tmp_6 = (Mktuple__16 1 1 1 1 1 1 1 1 1 1 1 1 __tmp_19 "hello" false true) in 
-                  let x2 = __tmp_6 in 
-                    let y = 20 in 
-                      let __tmp_26 = (nSMain__identityUnion y) in 
-                        let y2 = __tmp_26 in 
-                          let _MIRAccessFromIndex = 0 in 
-                            let __tmp_28 = (nSMain__max __tmp_31 y) in 
-                              let z = __tmp_28 in 
-                                let __tmp_33 = (nSMain__max z y) in 
-                                  let z_max_func_repeated = __tmp_33 in 
-                                    let __tmp_37 = (Mktuple__3 1 true 2) in 
-                                      let __tmp_36 = (nSMain__identityTupleOptional __tmp_37) in 
-                                        let z2 = __tmp_36 in 
-                                          let __tmp_42 = (Mktuple__1 "hello") in 
-                                            let __tmp_41 = (nSMain__identityOpenTuple __tmp_42) in 
-                                              let z3 = __tmp_41 in 
-                                                let __tmp_44 = (nSMain__maxx false 3) in 
-                                                  let z4 = __tmp_44 in 
-                                                    let __tmp_47 = (Mktuple__2 xTuple2 y) in 
-                                                      let zTuple2 = __tmp_47 in 
-                                                        let __ir_ret__ = z in 
-                                                          let _return_ = __ir_ret__ in 
-                                                            _return_
+  let string_test = (BTypedString "string_test" BAnyType) in 
+    let __tmp_6 = (BnSMain__PlayerMark (BTypedString "o" BAnyType)) in 
+      let __tmp_1 = (BnSMain__Artist (BInt 100) (BBool true) (BTypedString "Cornell" BAnyType) (BTypedString "Chris" BAnyType) __tmp_6) in 
+        let node = __tmp_1 in 
+          let __tmp_8 = (BnSMain__PlayerMark (BTypedString "x" BAnyType)) in 
+            let player1 = __tmp_8 in 
+              let __tmp_10 = (BInt 0) in 
+                let player2 = __tmp_10 in 
+                  let __tmp_11 = (BnSMain__Artist (BInt 100) (BBool true) (BTypedString "Pan" BAnyType) (BTypedString "Peter" BAnyType) player1) in 
+                    let node1 = __tmp_11 in 
+                      let __tmp_17 = (BnSMain__Artist (BInt 100) (BBool true) (BTypedString "Cornell" BAnyType) (BTypedString "Chris" BAnyType) player1) in 
+                        let node2 = __tmp_17 in 
+                          let n = BNone in 
+                            let __tmp_24 = (Mktuple__2 (BInt 10) (BInt 30)) in 
+                              let xTuple2 = __tmp_24 in 
+                                let __tmp_40 = (Mktuple__2 (BInt 1) (BInt 1)) in 
+                                  let __tmp_27 = (Mktuple__16 (BInt 1) (BInt 1) (BInt 1) (BInt 1) (BInt 1) (BInt 1) (BInt 1) (BInt 1) (BInt 1) (BInt 1) (BInt 1) (BInt 1) __tmp_40 (BTypedString "hello" BAnyType) (BBool false) (BBool true)) in 
+                                    let x2 = __tmp_27 in 
+                                      let y = (BInt 20) in 
+                                        let __tmp_47 = (nSMain__identityUnion y) in 
+                                          let y2 = __tmp_47 in 
+                                            let _MIRAccessFromIndex = (BInt 0) in 
+                                              let __tmp_49 = (nSMain__max __tmp_52 y) in 
+                                                let z = __tmp_49 in 
+                                                  let __tmp_54 = (nSMain__max z y) in 
+                                                    let z_max_func_repeated = __tmp_54 in 
+                                                      let __tmp_58 = (Mktuple__3 (BInt 1) (BBool true) (BInt 2)) in 
+                                                        let __tmp_57 = (nSMain__identityTupleOptional __tmp_58) in 
+                                                          let z2 = __tmp_57 in 
+                                                            let __tmp_63 = (Mktuple__1 (BTypedString "hello" BAnyType)) in 
+                                                              let __tmp_62 = (nSMain__identityOpenTuple __tmp_63) in 
+                                                                let z3 = __tmp_62 in 
+                                                                  let __tmp_65 = (nSMain__maxx (BBool false) (BInt 3)) in 
+                                                                    let z4 = __tmp_65 in 
+                                                                      let __tmp_68 = (Mktuple__2 xTuple2 y) in 
+                                                                        let zTuple2 = __tmp_68 in 
+                                                                          let __ir_ret__ = z in 
+                                                                            let _return_ = __ir_ret__ in 
+                                                                              _return_
 
